Added typing for STLC expressions, modified free_vars_indx function to return list of free vars and number of binders (possibly use this information in backtranslation function?), commented out rest of code that would need to be changed for new free_vars_indx function to work

rupicola/stlc_v2/STLC.fst
@@ -6,6 +6,12 @@ open FStar.Tactics
 open FStar.Classical.Sugar
 open FStar.List.Tot
 
+type typ =
+  | TUnit  : typ 
+  | TBool  : typ 
+  | TArr   : typ -> typ -> typ
+  | TPair  : typ -> typ -> typ
+
 let var = nat
 type exp =
   | EUnit  : exp
@@ -86,23 +92,26 @@ let sub_beta (e:exp)
          with 0 and ();
     f
 
-let rec free_vars_indx (e:exp) (n:nat) : list var = // n is the number of binders
+let rec free_vars_indx (e:exp) (n:nat) : (list var * nat) = // n is the number of binders
   match e with
-  | EUnit -> []
-  | ETrue -> []
-  | EFalse -> []
+  | EUnit -> ([], n)
+  | ETrue -> ([], n)
+  | EFalse -> ([], n)
   | ELam e' -> free_vars_indx e' (n+1)
-  | EApp e1 e2 -> free_vars_indx e1 n @ free_vars_indx e2 n
-  | EIf e1 e2 e3 -> free_vars_indx e1 n @ free_vars_indx e2 n @ free_vars_indx e3 n
-  | EVar i -> if i < n then [] else [i-n]
-  | EPair e1 e2 -> free_vars_indx e1 n @ free_vars_indx e2 n
+  | EApp e1 e2 -> (fst (free_vars_indx e1 n) @ fst (free_vars_indx e2 n), snd (free_vars_indx e1 n) + snd (free_vars_indx e2 n))
+  | EIf e1 e2 e3 -> (fst (free_vars_indx e1 n) @ fst (free_vars_indx e2 n) @ fst (free_vars_indx e3 n), snd (free_vars_indx e1 n) + snd (free_vars_indx e2 n) + snd (free_vars_indx e3 n))
+  | EVar i -> if i < n then ([], n) else ([i-n], n)
+  | EPair e1 e2 -> (fst (free_vars_indx e1 n) @ fst (free_vars_indx e2 n), snd (free_vars_indx e1 n) + snd (free_vars_indx e2 n))
   | EFst e' -> free_vars_indx e' n
   | ESnd e' -> free_vars_indx e' n
 
 let free_vars e = free_vars_indx e 0
 
 let is_closed (e:exp) : bool =
-  free_vars e = []
+  let (ls, _) = free_vars e in
+  ls = []
+
+let _ = assert (free_vars (ELam(ELam(EVar 0))) == ([], 2)) 
 
 let rec is_value (e:exp) : Type0 =
   match e with
@@ -124,11 +133,11 @@ let rec lem_value_is_closed (e:exp) : Lemma
 type value = e:exp{is_value e}
 type closed_exp = e:exp{is_closed e}
 
-let rec lem_shifting_preserves_closed (s:sub true) (e:exp) (n:nat) :
+(*let rec lem_shifting_preserves_closed (s:sub true) (e:exp) (n:nat) :
   Lemma
     (requires (free_vars_indx e n == [] /\
                (forall (x:var). EVar?.v (s x) <= x+1)))
-    (ensures (free_vars_indx (subst s e) (n+1) == []))
+    (ensures (fst (free_vars_indx (subst s e) (n+1)) == []))
     (decreases e) =
   match e with
   | ELam e' -> begin
@@ -421,3 +430,4 @@ let lem_destruct_steps_epair_snd
   (e':closed_exp) :
   Lemma (requires (steps (ESnd (EPair e1 e2)) e' /\ irred e1 /\ irred e2))
         (ensures (e2 == e')) = admit ()
+        *)
